proof of lemma monotonic_futures

Casper.thy
@@ -4,6 +4,7 @@ imports Main
 
 begin
 
+(* Section 2: Description of CBC Casper *)
 (* Section 2.1: CBC Casper "Parameters" *)
 
 (* Definition 2.1 *)
@@ -46,20 +47,20 @@ fun justification :: "message \<Rightarrow> state"
     "justification (Message (_, _, ml)) = set ml"
 
 (* Definition 2.7 *)
-(* NOTE: Why "fun" instead of "definition" ?  *)
 fun is_valid :: "weight \<Rightarrow>(estimator \<Rightarrow> (message \<Rightarrow> bool))"
   where
     "is_valid w e (Message (c, v, s)) = (c = e w (set s))"
 
+(* FIXME: Can we construct valid_message type? Currently we assume all states are valid in all the 
+"definition"s and use is_valid_state for all occurrences of state type in lemmas. *)
 definition is_valid_state :: "weight \<Rightarrow> estimator \<Rightarrow> state \<Rightarrow> bool"
   where
     "is_valid_state w e s = (\<forall> m \<in> s. is_valid w e m)"
 
 (* Definition 2.8: Protocol state transitions \<rightarrow> *)
-definition is_future_state :: "weight \<Rightarrow> estimator \<Rightarrow> state \<Rightarrow> state \<Rightarrow> bool"
+definition is_future_state :: "state \<Rightarrow> state \<Rightarrow> bool"
   where
-    "is_future_state w e s0 s1 =
-      (s0 \<supseteq> s1 \<and> is_valid_state w e s0 \<and> is_valid_state w e s1)"
+    "is_future_state s0 s1 = (s0 \<supseteq> s1)"
 
 (* Definition 2.9 *)
 definition equivocation :: "message \<Rightarrow> message \<Rightarrow> bool"
@@ -68,11 +69,10 @@ definition equivocation :: "message \<Rightarrow> message \<Rightarrow> bool"
       (sender m0 = sender m1 \<and> m0 \<noteq> m1 \<and> m0 \<notin> justification(m1) \<and> m1 \<notin> justification(m0))"
 
 (* Definition 2.10 *)
-(* FIXME: Existence of multiple variables?  *)
 definition equivocating_validators :: "state \<Rightarrow> validator set"
   where
     "equivocating_validators s = 
-      {v. \<exists> m0. m0 \<in> s \<and> (\<exists> m1. m1 \<in> s \<and> equivocation m0 m1 \<and> sender m0 = v)}"
+      {v. \<exists> m0 m1. m0 \<in> s \<and> m1 \<in> s \<and> equivocation m0 m1 \<and> sender m0 = v}"
 
 (* Definition 2.11 *)
 definition equivocation_fault_weight :: "weight \<Rightarrow> state \<Rightarrow> int"
@@ -80,8 +80,23 @@ definition equivocation_fault_weight :: "weight \<Rightarrow> state \<Rightarrow
     "equivocation_fault_weight w s = sum w (equivocating_validators s)"
 
 (* Definition 2.12 *)
-definition is_faults_lt_threshold :: "weight \<Rightarrow> threshold \<Rightarrow> state \<Rightarrow> bool"
+definition is_faults_lt_threshold :: "threshold \<Rightarrow> weight \<Rightarrow> state \<Rightarrow> bool"
   where 
-    "is_faults_lt_threshold w t s = (equivocation_fault_weight w s < t)"
+    "is_faults_lt_threshold t w s = (equivocation_fault_weight w s < t)"
+
+(* Section 3: Safety Proof *)
+(* Section 3.1: Guaranteeing Common Futures *)
+
+(* Definition 3.1 *)
+definition futures :: "threshold \<Rightarrow> weight \<Rightarrow> state \<Rightarrow> state set"
+  where
+    "futures t w s = {s'. is_faults_lt_threshold t w s' \<and> is_future_state s' s}"
+
+(* Lemma 1 *)
+lemma monotonic_futures :
+  "\<forall> s' s. is_faults_lt_threshold t w s' \<and> is_faults_lt_threshold t w s
+   \<and> is_valid_state w e s' \<and> is_valid_state w e s
+   \<Longrightarrow> (s' \<in> futures t w s \<longleftrightarrow> futures t w s' \<subseteq> futures t w s)"
+   using futures_def is_future_state_def by auto
 
 end
